zoo_parabs: Move futures to a new separate module.

lib/examples/fibonacci.ml
@@ -2,8 +2,8 @@ let rec fibonacci n ctx =
   if n <= 1 then
     n
   else
-    let fut1 = Pool.async ctx (fun ctx -> fibonacci (n - 1) ctx) in
-    let fut2 = Pool.async ctx (fun ctx -> fibonacci (n - 2) ctx) in
-    Pool.wait ctx fut1 + Pool.wait ctx fut2
+    let fut1 = Future.async ctx (fun ctx -> fibonacci (n - 1) ctx) in
+    let fut2 = Future.async ctx (fun ctx -> fibonacci (n - 2) ctx) in
+    Future.wait ctx fut1 + Future.wait ctx fut2
 let fibonacci n pool =
   Pool.run pool (fun ctx -> fibonacci n ctx)
