lib/zoo_parabs/algo.ml
@@ -7,7 +7,7 @@ let for_ ctx beg end_ chunk fn =
   let num_task = num_chunk + Bool.to_int (rest != 0) in
   let num_pending = Atomic.make num_task in
   for i = 0 to num_chunk - 1 do
-    Pool.async_silent ctx (fun ctx ->
+    Pool.async ctx (fun ctx ->
       for k = i * chunk to i * chunk + chunk - 1 do
         fn ctx k
       done ;
@@ -15,7 +15,7 @@ let for_ ctx beg end_ chunk fn =
     )
   done ;
   if rest != 0 then
-    Pool.async_silent ctx (fun ctx ->
+    Pool.async ctx (fun ctx ->
       for k = num_chunk * chunk to end_ - 1 do
         fn ctx k
       done ;
@@ -25,15 +25,17 @@ let for_ ctx beg end_ chunk fn =
 
 let rec for_2 ctx beg end_ chunk fn =
   if end_ - beg <= chunk then
-    for i = beg to end_ - 1 do fn ctx i done
-  else begin
+    for i = beg to end_ - 1 do
+      fn ctx i
+    done
+  else
     let mid = beg + (end_ - beg) / 2 in
-    let left = Pool.async ctx (fun ctx ->
-      for_2 ctx beg mid chunk fn
-    ) in
-    for_2 ctx mid end_ chunk fn;
-    Pool.wait ctx left
-  end
+    let left =
+      Future.async ctx @@ fun ctx ->
+        for_2 ctx beg mid chunk fn
+    in
+    for_2 ctx mid end_ chunk fn ;
+    Future.wait ctx left
 
 let divide ctx beg end_ fn =
   let num_dom = Pool.size ctx + 1 in
@@ -43,13 +45,13 @@ let divide ctx beg end_ fn =
   let num_task = num_dom + Bool.to_int (rest != 0) in
   let num_pending = Atomic.make num_task in
   for i = 0 to num_dom - 1 do
-    Pool.async_silent ctx (fun ctx ->
+    Pool.async ctx (fun ctx ->
       fn ctx (i * chunk) chunk ;
       Atomic.decr num_pending
     )
   done ;
   if rest != 0 then
-    Pool.async_silent ctx (fun ctx ->
+    Pool.async ctx (fun ctx ->
       fn ctx (num_dom * chunk) rest ;
       Atomic.decr num_pending
     ) ;
@@ -70,14 +72,14 @@ let fold ctx beg end_ chunk op body zero =
   let num_pending = Atomic.make num_task in
   let sums = Array.make num_task zero in
   for i = 0 to num_chunk - 1 do
-    Pool.async_silent ctx (fun ctx ->
+    Pool.async ctx (fun ctx ->
       let sum = fold ctx op body zero (i * chunk) ((i + 1) * chunk) in
       Array.unsafe_set sums i sum ;
       Atomic.decr num_pending
     )
   done ;
   if rest != 0 then
-    Pool.async_silent ctx (fun ctx ->
+    Pool.async ctx (fun ctx ->
       let sum = fold ctx op body zero (num_chunk * chunk) end_ in
       Array.unsafe_set sums num_chunk sum ;
       Atomic.decr num_pending
@@ -101,13 +103,13 @@ let find ctx beg end_ chunk pred =
   let num_pending = Atomic.make num_task in
   let found = ref None in
   for i = 0 to num_chunk - 1 do
-    Pool.async_silent ctx (fun ctx ->
+    Pool.async ctx (fun ctx ->
       find ctx (i * chunk) ((i + 1) * chunk) pred found ;
       Atomic.decr num_pending
     )
   done ;
   if rest != 0 then
-    Pool.async_silent ctx (fun ctx ->
+    Pool.async ctx (fun ctx ->
       find ctx (num_chunk * chunk) end_ pred found ;
       Atomic.decr num_pending
     ) ;
