lib/zoo_parabs/future.ml
@@ -1,0 +1,31 @@
+type 'a t =
+  ('a, ('a -> unit) Pool.task) Ivar_3.t
+
+let async ctx task =
+  let t = Ivar_3.create () in
+  Pool.async ctx (fun ctx ->
+    let res = task ctx in
+    let waiters = Ivar_3.set t res in
+    Lst.iter (fun waiter -> waiter ctx res) waiters
+  ) ;
+  t
+
+let wait ctx t =
+  Pool.wait_until ctx (fun () -> Ivar_3.is_set t) ;
+  Ivar_3.get t
+
+let iter ctx t fn =
+  match Ivar_3.wait t fn with
+  | None ->
+      ()
+  | Some res ->
+      fn ctx res
+
+let map ctx t1 fn =
+  let t2 = Ivar_3.create () in
+  iter ctx t1 (fun ctx res1 ->
+    let res2 = fn ctx res1 in
+    let waiters = Ivar_3.set t2 res2 in
+    Lst.iter (fun waiter -> waiter ctx res2) waiters
+  ) ;
+  t2
