lib/zoo_parabs/future.mli
@@ -1,0 +1,13 @@
+type 'a t
+
+val async :
+  Pool.context -> 'a Pool.task -> 'a t
+
+val wait :
+  Pool.context -> 'a t -> 'a
+
+val iter :
+  Pool.context -> 'a t -> ('a -> unit) Pool.task -> unit
+
+val map :
+  Pool.context -> 'a t -> ('a -> 'b) Pool.task -> 'b t
