lib/zoo_parabs/pool.mli
@@ -5,8 +5,6 @@ type context
 type 'a task =
   context -> 'a
 
-type 'a future
-
 val create :
   int -> t
 
@@ -19,21 +17,10 @@ val kill :
 val size :
   context -> int
 
-val async_silent :
-  context -> unit task -> unit
 val async :
-  context -> 'a task -> 'a future
+  context -> unit task -> unit
 
 val wait_until :
   context -> (unit -> bool) -> unit
 val wait_while :
   context -> (unit -> bool) -> unit
-
-val wait :
-  context -> 'a future -> 'a
-
-val iter :
-  context -> 'a future -> ('a -> unit) task -> unit
-
-val map :
-  context -> 'a future -> ('a -> 'b) task -> 'b future
