theories/examples/fibonacci.v
@@ -5,6 +5,7 @@ From zoo.language Require Import
 From zoo.diaframe Require Import
   diaframe.
 From zoo_parabs Require Import
+  future
   pool.
 From examples Require Export
   fibonacci__code.
@@ -50,18 +51,18 @@ Proof.
   apply decide_ext. lia.
 Qed.
 
-Section pool_G.
-  Context `{pool_G : SchedulerG Σ}.
+Section future_G.
+  Context `{future_G : FutureG Σ}.
 
-  #[local] Lemma fibonacci_fibonacci_0_spec n t ctx scope :
+  #[local] Lemma fibonacci_fibonacci_0_spec n pool ctx scope :
     (0 ≤ n)%Z →
     {{{
-      pool_context t ctx scope
+      pool_context pool ctx scope
     }}}
       fibonacci_fibonacci_0 #n ctx
     {{{
       RET #(fib ₊n);
-      pool_context t ctx scope
+      pool_context pool ctx scope
     }}}.
   Proof.
     iLöb as "HLöb" forall (n ctx scope).
@@ -73,18 +74,18 @@ Section pool_G.
 
     - assert (n = 0 ∨ n = 1) as [-> | ->] by lia; iSteps.
 
-    - wp_apply (pool_async_spec (λ v1, ⌜v1 = #_⌝)%I (λ _, True)%I with "[$Hctx]") as (fut1) "(Hctx & #Hfut1_inv & Hfut1_consumer & _)".
+    - wp_apply (future_async_spec (λ v1, ⌜v1 = #_⌝)%I (λ _, True)%I pool _ scope with "[$Hctx]") as (fut1) "(Hctx & #Hfut1_inv & Hfut1_consumer & _)".
       { clear ctx scope. iIntros "%ctx %scope Hctx".
         wp_smart_apply ("HLöb" with "[] Hctx"); iSteps.
       }
-      wp_smart_apply (pool_async_spec (λ v2, ⌜v2 = #_⌝)%I (λ _, True)%I with "[$Hctx]") as (fut2) "(Hctx & #Hfut2_inv & Hfut2_consumer & _)".
+      wp_smart_apply (future_async_spec (λ v2, ⌜v2 = #_⌝)%I (λ _, True)%I with "[$Hctx]") as (fut2) "(Hctx & #Hfut2_inv & Hfut2_consumer & _)".
       { clear ctx scope. iIntros "%ctx %scope Hctx".
         wp_smart_apply ("HLöb" with "[] Hctx"); iSteps.
       }
-      wp_smart_apply (pool_wait_spec with "[$Hctx $Hfut2_inv]") as (?) "(H£ & Hctx & Hfut2_result)".
-      iMod (pool_future_inv_result_consumer' with "H£ Hfut2_inv Hfut2_result Hfut2_consumer") as "(-> & _)".
-      wp_smart_apply (pool_wait_spec with "[$Hctx $Hfut1_inv]") as (?) "(H£ & Hctx & Hfut1_result)".
-      iMod (pool_future_inv_result_consumer' with "H£ Hfut1_inv Hfut1_result Hfut1_consumer") as "(-> & _)".
+      wp_smart_apply (future_wait_spec with "[$Hctx $Hfut2_inv]") as (?) "(H£ & Hctx & Hfut2_result)".
+      iMod (future_inv_result_consumer' with "H£ Hfut2_inv Hfut2_result Hfut2_consumer") as "(-> & _)".
+      wp_smart_apply (future_wait_spec with "[$Hctx $Hfut1_inv]") as (?) "(H£ & Hctx & Hfut1_result)".
+      iMod (future_inv_result_consumer' with "H£ Hfut1_inv Hfut1_result Hfut1_consumer") as "(-> & _)".
       wp_pures.
       rewrite (fib_spec_Z n) // -Nat2Z.inj_add.
       rewrite decide_False; first lia.
@@ -106,7 +107,7 @@ Section pool_G.
     wp_smart_apply (fibonacci_fibonacci_0_spec with "Hctx"); first lia.
     rewrite Nat2Z.id. iSteps.
   Qed.
-End pool_G.
+End future_G.
 
 From examples Require
   fibonacci__opaque.
