theories/zoo_parabs/future.v
@@ -1,0 +1,307 @@
+From zoo Require Import
+  prelude.
+From zoo.iris.bi Require Import
+  big_op.
+From zoo.language Require Import
+  notations.
+From zoo.diaframe Require Import
+  diaframe.
+From zoo_std Require Import
+  ivar_3
+  lst.
+From zoo_parabs Require Export
+  base
+  future__code.
+From zoo_parabs Require Import
+  pool.
+From zoo Require Import
+  options.
+
+Implicit Types b : bool.
+Implicit Types v t pool ctx task waiter fn : val.
+Implicit Types scope : pool_scope.
+Implicit Types ω : unit.
+
+Class FutureG Σ `{pool_G : PoolG Σ} := {
+  #[local] future_G_ivar_G :: Ivar3G Σ unit ;
+}.
+
+Definition future_Σ := #[
+  ivar_3_Σ unit
+].
+#[global] Instance subG_future_Σ Σ `{pool_G : PoolG Σ} :
+  subG future_Σ Σ →
+  FutureG Σ.
+Proof.
+  solve_inG.
+Qed.
+
+Section future_G.
+  Context `{future_G : FutureG Σ}.
+
+  Implicit Types Ψ Χ Ξ : val → iProp Σ.
+
+  #[local] Definition waiter_model pool t waiter ω : iProp Σ :=
+    ∀ ctx scope v,
+    pool_context pool ctx scope -∗
+    ivar_3_result t v -∗
+    WP waiter ctx v {{ res,
+      ⌜res = ()%V⌝ ∗
+      pool_context pool ctx scope
+    }}.
+  Definition future_inv pool t Ψ Ξ :=
+    ivar_3_inv t Ψ Ξ (waiter_model pool).
+
+  Definition future_consumer :=
+    ivar_3_consumer.
+
+  Definition future_result :=
+    ivar_3_result.
+  Definition future_finished t : iProp Σ :=
+    ∃ v,
+    future_result t v.
+
+  #[global] Instance future_proper pool t :
+    Proper (
+      (pointwise_relation _ (≡)) ==>
+      (pointwise_relation _ (≡)) ==>
+      (≡)
+    ) (future_inv pool t).
+  Proof.
+    solve_proper.
+  Qed.
+
+  #[global] Instance future_result_timeless t v :
+    Timeless (future_result t v).
+  Proof.
+    apply _.
+  Qed.
+
+  #[global] Instance future_inv_persistent pool t Ψ Ξ :
+    Persistent (future_inv pool t Ψ Ξ).
+  Proof.
+    apply _.
+  Qed.
+  #[global] Instance future_result_persistent t v :
+    Persistent (future_result t v).
+  Proof.
+    apply _.
+  Qed.
+
+  Lemma future_consumer_divide {pool t Ψ Ξ Χ} Χs :
+    future_inv pool t Ψ Ξ -∗
+    future_consumer t Χ -∗
+    (∀ x, Χ x -∗ [∗ list] Χ ∈ Χs, Χ x) ={⊤}=∗
+    [∗ list] Χ ∈ Χs, future_consumer t Χ.
+  Proof.
+    apply ivar_3_consumer_divide.
+  Qed.
+  Lemma future_consumer_split {pool t Ψ Χ Ξ} Χ1 Χ2 :
+    future_inv pool t Ψ Ξ -∗
+    future_consumer t Χ -∗
+    (∀ v, Χ v -∗ Χ1 v ∗ Χ2 v) ={⊤}=∗
+      future_consumer t Χ1 ∗
+      future_consumer t Χ2.
+  Proof.
+    apply ivar_3_consumer_split.
+  Qed.
+
+  Lemma future_result_agree t v1 v2 :
+    future_result t v1 -∗
+    future_result t v2 -∗
+    ⌜v1 = v2⌝.
+  Proof.
+    apply ivar_3_result_agree.
+  Qed.
+
+  Lemma future_inv_result pool t Ψ Ξ v :
+    future_inv pool t Ψ Ξ -∗
+    future_result t v ={⊤}=∗
+    ▷ □ Ξ v.
+  Proof.
+    apply ivar_3_inv_result.
+  Qed.
+  Lemma future_inv_result' pool t Ψ Ξ v :
+    £ 1 -∗
+    future_inv pool t Ψ Ξ -∗
+    future_result t v ={⊤}=∗
+    □ Ξ v.
+  Proof.
+    iIntros "H£ Hfut_inv Hfut_result".
+    iMod (future_inv_result with "Hfut_inv Hfut_result") as "HΞ".
+    iApply (lc_fupd_elim_later with "H£ HΞ").
+  Qed.
+  Lemma future_inv_result_consumer pool t Ψ Ξ v Χ :
+    future_inv pool t Ψ Ξ -∗
+    future_result t v -∗
+    future_consumer t Χ ={⊤}=∗
+      ▷^2 Χ v ∗
+      ▷ □ Ξ v.
+  Proof.
+    apply ivar_3_inv_result_consumer.
+  Qed.
+  Lemma future_inv_result_consumer' pool t Ψ Ξ v Χ :
+    £ 2 -∗
+    future_inv pool t Ψ Ξ -∗
+    future_result t v -∗
+    future_consumer t Χ ={⊤}=∗
+      Χ v ∗
+      □ Ξ v.
+  Proof.
+    iIntros "(H£1 & H£2) Hfut_inv Hfut_result Hfut_consumer".
+    iMod (future_inv_result_consumer with "Hfut_inv Hfut_result Hfut_consumer") as "H".
+    rewrite -bi.later_sep.
+    iMod (lc_fupd_elim_later with "H£1 H") as "(HΧ & $)".
+    iApply (lc_fupd_elim_later with "H£2 HΧ").
+  Qed.
+
+  Lemma future_async_spec Ψ Ξ pool ctx scope task :
+    {{{
+      pool_context pool ctx scope ∗
+      ( ∀ ctx scope,
+        pool_context pool ctx scope -∗
+        WP task ctx {{ v,
+          pool_context pool ctx scope ∗
+          ▷ Ψ v ∗
+          ▷ □ Ξ v
+        }}
+      )
+    }}}
+      future_async ctx task
+    {{{ t,
+      RET t;
+      pool_context pool ctx scope ∗
+      future_inv pool t Ψ Ξ ∗
+      future_consumer t Ψ ∗
+      pool_obligation pool (future_finished t)
+    }}}.
+  Proof.
+    iIntros "%Φ (Hctx & Htask) HΦ".
+
+    wp_rec.
+    wp_smart_apply (ivar_3_create_spec Ψ Ξ with "[//]") as (ivar) "(#Hivar_inv & Hivar_producer & Hivar_consumer)".
+
+    wp_smart_apply (pool_async_spec (
+      ivar_3_resolved ivar
+    ) with "[$Hctx Htask Hivar_producer]") as "(Hctx & Hobligation)".
+    { clear ctx scope. iIntros "%ctx %scope Hctx".
+
+      wp_smart_apply (wp_wand with "(Htask Hctx)") as (v) "(Hctx & HΨ & HΞ)".
+      wp_smart_apply (ivar_3_set_spec with "[$Hivar_inv $Hivar_producer $HΨ $HΞ]") as (waiters ωs) "(#Hivar_result & _ & Hwaiters)".
+
+      wp_smart_apply (lst_iter_spec' (λ _ _, pool_context pool ctx scope)%I with "[$Hctx Hwaiters]") as "$"; first done.
+      { iDestruct (big_sepL2_retract_r with "Hwaiters") as "(_ & Hwaiters)".
+        iApply (big_sepL_impl with "Hwaiters").
+        iSteps.
+      }
+
+      iFrame "#∗".
+    }
+
+    iSteps.
+  Qed.
+
+  Lemma future_wait_spec pool ctx scope t Ψ Ξ :
+    {{{
+      pool_context pool ctx scope ∗
+      future_inv pool t Ψ Ξ
+    }}}
+      future_wait ctx t
+    {{{ v,
+      RET v;
+      £ 2 ∗
+      pool_context pool ctx scope ∗
+      future_result t v
+    }}}.
+  Proof.
+    iIntros "%Φ (Hctx & #Hivar_inv) HΦ".
+
+    wp_rec.
+
+    wp_smart_apply (pool_wait_until_spec (ivar_3_resolved t)%I with "[$Hctx]") as "(Hctx & %v & #Hivar_result)".
+    { iModIntro.
+      wp_smart_apply (ivar_3_is_set_spec with "Hivar_inv") as (b) "Hivar_result".
+      rewrite /ivar_3_resolved. destruct b; iSteps.
+    }
+
+    wp_smart_apply (ivar_3_get_spec with "[$Hivar_inv $Hivar_result]") as "H£".
+    iSteps.
+  Qed.
+
+  Lemma future_iter_spec pool ctx scope t Ψ Ξ fn :
+    {{{
+      pool_context pool ctx scope ∗
+      future_inv pool t Ψ Ξ ∗
+      ( ∀ ctx scope v,
+        pool_context pool ctx scope -∗
+        future_result t v -∗
+        WP fn ctx v {{ res,
+          ⌜res = ()%V⌝ ∗
+          pool_context pool ctx scope
+        }}
+      )
+    }}}
+      future_iter ctx t fn
+    {{{
+      RET ();
+      pool_context pool ctx scope
+    }}}.
+  Proof.
+    iIntros "%Φ (Hctx & #Hivar_inv & Hfn) HΦ".
+
+    wp_rec.
+    wp_smart_apply (ivar_3_wait_spec inhabitant with "[$Hivar_inv $Hfn]") as ([v |]) "H"; iSteps.
+  Qed.
+
+  Lemma future_map_spec {pool ctx scope t1 Ψ1 Ξ1} Ψ2 Ξ2 fn :
+    {{{
+      pool_context pool ctx scope ∗
+      future_inv pool t1 Ψ1 Ξ1 ∗
+      ( ∀ ctx scope v1,
+        pool_context pool ctx scope -∗
+        future_result t1 v1 -∗
+        WP fn ctx v1 {{ v2,
+          pool_context pool ctx scope ∗
+          ▷ Ψ2 v2 ∗
+          ▷ □ Ξ2 v2
+        }}
+      )
+    }}}
+      future_map ctx t1 fn
+    {{{ t2,
+      RET t2;
+      pool_context pool ctx scope ∗
+      future_inv pool t2 Ψ2 Ξ2 ∗
+      future_consumer t2 Ψ2
+    }}}.
+  Proof.
+    iIntros "%Φ (Hctx & #Ht1_inv & Hfn) HΦ".
+
+    wp_rec.
+    wp_smart_apply (ivar_3_create_spec Ψ2 Ξ2 with "[//]") as (t2) "(#Hivar2_inv & Hivar2_producer & Hivar2_consumer)".
+
+    wp_smart_apply (future_iter_spec with "[$Hctx $Ht1_inv Hfn Hivar2_producer]") as "Hctx".
+    { clear ctx scope. iIntros "%ctx %scope %v1 Hctx #Ht1_result".
+
+      wp_smart_apply (wp_wand with "(Hfn Hctx Ht1_result)") as (v2) "(Hctx & HΨ2 & HΞ2)".
+      wp_smart_apply (ivar_3_set_spec with "[$Hivar2_inv $Hivar2_producer $HΨ2 $HΞ2]") as (waiters ωs) "(#Hivar2_result & _ & Hwaiters)".
+
+      wp_smart_apply (lst_iter_spec' (λ _ _, pool_context pool ctx scope)%I with "[$Hctx Hwaiters]") as "$"; first done.
+      { iDestruct (big_sepL2_retract_r with "Hwaiters") as "(_ & Hwaiters)".
+        iApply (big_sepL_impl with "Hwaiters").
+        iSteps.
+      }
+
+      iSteps.
+    }
+
+    iSteps.
+  Qed.
+End future_G.
+
+From zoo_parabs Require
+  future__opaque.
+
+#[global] Opaque future_inv.
+#[global] Opaque future_consumer.
+#[global] Opaque future_result.
