theories/zoo_parabs/future__code.v
@@ -1,0 +1,51 @@
+From zoo Require Import
+  prelude.
+From zoo.language Require Import
+  typeclasses
+  notations.
+From zoo_std Require Import
+  lst
+  ivar_3.
+From zoo_parabs Require Import
+  pool.
+From zoo_parabs Require Import
+  future__types.
+From zoo Require Import
+  options.
+
+Definition future_async : val :=
+  fun: "ctx" "task" =>
+    let: "t" := ivar_3_create () in
+    pool_async
+      "ctx"
+      (fun: "ctx" =>
+         let: "res" := "task" "ctx" in
+         let: "waiters" := ivar_3_set "t" "res" in
+         lst_iter (fun: "waiter" => "waiter" "ctx" "res") "waiters") ;;
+    "t".
+
+Definition future_wait : val :=
+  fun: "ctx" "t" =>
+    pool_wait_until "ctx" (fun: <> => ivar_3_is_set "t") ;;
+    ivar_3_get "t".
+
+Definition future_iter : val :=
+  fun: "ctx" "t" "fn" =>
+    match: ivar_3_wait "t" "fn" with
+    | None =>
+        ()
+    | Some "res" =>
+        "fn" "ctx" "res"
+    end.
+
+Definition future_map : val :=
+  fun: "ctx" "t1" "fn" =>
+    let: "t2" := ivar_3_create () in
+    future_iter
+      "ctx"
+      "t1"
+      (fun: "ctx" "res1" =>
+         let: "res2" := "fn" "ctx" "res1" in
+         let: "waiters" := ivar_3_set "t2" "res2" in
+         lst_iter (fun: "waiter" => "waiter" "ctx" "res2") "waiters") ;;
+    "t2".
