theories/zoo_parabs/future__opaque.v
@@ -1,0 +1,7 @@
+From zoo_parabs Require Import
+  future__code.
+
+#[global] Opaque future_async.
+#[global] Opaque future_wait.
+#[global] Opaque future_iter.
+#[global] Opaque future_map.
