theories/zoo_parabs/future__types.v
@@ -3,8 +3,10 @@ From zoo Require Import
 From zoo.language Require Import
   typeclasses
   notations.
+From zoo_std Require Import
+  lst
+  ivar_3.
 From zoo_parabs Require Import
-  future
   pool.
 From zoo Require Import
   options.
