theories/zoo_parabs/pool__opaque.v
@@ -5,10 +5,6 @@ From zoo_parabs Require Import
 #[global] Opaque pool_run.
 #[global] Opaque pool_kill.
 #[global] Opaque pool_size.
-#[global] Opaque pool_async_silent.
 #[global] Opaque pool_async.
 #[global] Opaque pool_wait_until.
 #[global] Opaque pool_wait_while.
-#[global] Opaque pool_wait.
-#[global] Opaque pool_iter.
-#[global] Opaque pool_map.
