theories/zoo_parabs/pool__types.v
@@ -4,8 +4,6 @@ From zoo.language Require Import
   typeclasses
   notations.
 From zoo_std Require Import
-  lst
-  ivar_3
   array
   domain.
 From zoo_parabs Require Import
